FreydSSA/Terminator/Fun/Subst.lean
@@ -24,17 +24,19 @@ inductive FLCtx.PSubstBot
 
 theorem FLCtx.PSubstBot.bot_mp {Γ : WithBot (FLabel ν (Ty α))} {σ : USubst φ ν} {Δ : WithBot (FLabel ν (Ty α))}
   (hσ : PSubstBot Γ σ Δ) : Γ = ⊥ → Δ = ⊥
-  := λh => by
-    cases hσ with
-    | bot => rfl
-    | subst => cases h
+  := λh => by cases hσ <;> simp at *
 
 theorem FLCtx.PSubstBot.bot_mpr {Γ : WithBot (FLabel ν (Ty α))} {σ : USubst φ ν} {Δ : WithBot (FLabel ν (Ty α))}
   (hσ : PSubstBot Γ σ Δ) : Δ = ⊥ → Γ = ⊥
-  := λh => by
-    cases hσ with
-    | bot => rfl
-    | subst => cases h
+  := λh => by cases hσ <;> simp at *
+
+theorem FLCtx.PSubstBot.is_some_mp {Γ : WithBot (FLabel ν (Ty α))} {σ : USubst φ ν} {Δ : WithBot (FLabel ν (Ty α))}
+  (hσ : PSubstBot Γ σ Δ) : Γ.isSome → Δ.isSome
+  := λh => by cases hσ <;> simp [Option.isSome] at *
+
+theorem FLCtx.PSubstBot.is_some_mpr {Γ : WithBot (FLabel ν (Ty α))} {σ : USubst φ ν} {Δ : WithBot (FLabel ν (Ty α))}
+  (hσ : PSubstBot Γ σ Δ) : Δ.isSome → Γ.isSome
+  := λh => by cases hσ <;> simp [Option.isSome] at *
 
 theorem FLCtx.PSubstBot.param_eq {Γ : FLabel ν (Ty α)} {σ : USubst φ ν} {Δ : FLabel ν (Ty α)}
   (hσ : @PSubstBot _ ν α Φ (↑Γ) σ (↑Δ)) : Γ.param = Δ.param
@@ -57,42 +59,82 @@ theorem FLCtx.PSubst.bot_mpr {L : FLCtx κ ν (Ty α)} {σ : USubst φ ν} {K : 
   (hσ : L.PSubst σ K) (x : κ) : K x = ⊥ → L x = ⊥
   := (hσ x).bot_mpr
 
--- def FLCtx.PSubst.lsup
---   {L₁ L₂ : FLCtx κ ν (Ty α)} {σ : USubst φ ν} {K₁ K₂ : FLCtx κ ν (Ty α)}
---   (hσ₁ : L₁.PSubst σ K₁) (hσ₂ : L₂.PSubst σ K₂) : (L₁.lsup L₂).PSubst σ (K₁.lsup K₂)
---   := λx => by
---     simp only [lsup_app, lsup_bot]
---     split
---     . rename_i he
---       split
---       . exact hσ₂ x
---       . rename_i c
---         exact (c $ hσ₁.bot_mp _ he).elim
---       . rename_i he' _
---         simp [hσ₁.bot_mp _ he] at he'
---     . rename_i he c
---       split
---       . rename_i he'
---         exact (c $ hσ₁.bot_mpr _ he').elim
---       . exact hσ₁ x
---       . rename_i he'
---         simp [hσ₂.bot_mp _ he] at he'
---     . rename_i Γ₁ Γ₂ hLe₁ hLe₂
---       split
---       . rename_i he
---         simp [hσ₁.bot_mpr _ he] at hLe₁
---       . rename_i he _
---         simp [hσ₂.bot_mpr _ he] at hLe₂
---       . rename_i Δ₁ Δ₂ hKe₁ hKe₂
---         let h₁ := hKe₁ ▸ hLe₁ ▸ hσ₁ x;
---         let h₂ := hKe₂ ▸ hLe₂ ▸ hσ₂ x;
---         cases h₁
---         constructor
---         sorry -- TODO: lsup substitution
---         assumption
---         -- apply PSubstBot.subst
+theorem FLCtx.PSubst.is_some_mp {L : FLCtx κ ν (Ty α)} {σ : USubst φ ν} {K : FLCtx κ ν (Ty α)}
+  (hσ : L.PSubst σ K) (x : κ) : (L x).isSome → (K x).isSome
+  := (hσ x).is_some_mp
 
--- TODO: PSubst preserves compatibility
+theorem FLCtx.PSubst.is_some_mpr {L : FLCtx κ ν (Ty α)} {σ : USubst φ ν} {K : FLCtx κ ν (Ty α)}
+  (hσ : L.PSubst σ K) (x : κ) : (K x).isSome → (L x).isSome
+  := (hσ x).is_some_mpr
+
+theorem FLCtx.PSubst.some_trg {L : FLCtx κ ν (Ty α)} {σ : USubst φ ν} {K : FLCtx κ ν (Ty α)}
+  (hσ : L.PSubst σ K) (x : κ) (Γ : FLabel ν (Ty α)) : L x = some Γ → Σ'Δ, K x = some Δ
+  := λh => ⟨(K x).get (hσ.is_some_mp x (by simp [h])), by simp⟩
+
+def FLCtx.PSubst.lsup
+  {L₁ L₂ : FLCtx κ ν (Ty α)} {σ : USubst φ ν} {K₁ K₂ : FLCtx κ ν (Ty α)}
+  (hσ₁ : L₁.PSubst σ K₁) (hσ₂ : L₂.PSubst σ K₂) (hL : L₁.Cmp L₂) : (L₁.lsup L₂).PSubst σ (K₁.lsup K₂)
+  := λx => by
+    simp only [lsup_app, lsup_bot]
+    split
+    . rename_i he
+      split
+      . exact hσ₂ x
+      . rename_i c
+        exact (c $ hσ₁.bot_mp _ he).elim
+      . rename_i he' _
+        simp [hσ₁.bot_mp _ he] at he'
+    . rename_i he c
+      split
+      . rename_i he'
+        exact (c $ hσ₁.bot_mpr _ he').elim
+      . exact hσ₁ x
+      . rename_i he'
+        simp [hσ₂.bot_mp _ he] at he'
+    . rename_i Γ₁ Γ₂ hLe₁ hLe₂
+      split
+      . rename_i he
+        simp [hσ₁.bot_mpr _ he] at hLe₁
+      . rename_i he _
+        simp [hσ₂.bot_mpr _ he] at hLe₂
+      . rename_i Δ₁ Δ₂ hKe₁ hKe₂
+        let h₁ := hKe₁ ▸ hLe₁ ▸ hσ₁ x;
+        let h₂ := hKe₂ ▸ hLe₂ ▸ hσ₂ x;
+        have hL := hLe₁ ▸ hLe₂ ▸ hL x
+        cases h₁ with
+        | subst hσ hparam =>
+          cases h₂ with
+          | subst hσ' hparam' =>
+            constructor
+            apply hσ.lsup hσ'
+            cases hL with
+            | both c => exact c.live
+            exact hparam
+
+-- theorem FCtx.Subst.cmp_label {Γ Δ Γ' Δ' : FLabel ν (Ty α)} {σ : USubst φ ν}
+--   (hσ : Γ.live.Subst σ Δ.live) (hσ' : Γ'.live.Subst σ Δ'.live) (hΓ : Γ.Cmp Γ') : Δ.Cmp Δ'
+--   := ⟨sorry, sorry⟩
+
+theorem FLCtx.PSubstBot.cmp
+  {Γ Δ Γ' Δ' : WithBot (FLabel ν (Ty α))} {σ : USubst φ ν}
+  (hσ : PSubstBot Γ σ Δ) (hσ' : PSubstBot Γ' σ Δ') (hΓ : FLCtx.CmpBot Γ Γ') : FLCtx.CmpBot Δ Δ'
+  := by
+    cases hσ with
+    | bot => constructor
+    | subst hΔ hp => cases hσ' with
+      | bot => constructor
+      | subst hΔ' hp' =>
+        cases hΓ with
+        | both hΓ =>
+          constructor
+          constructor
+          exact hΔ.cmp hΔ' hΓ.live
+          rw [<-hp, <-hp', hΓ.param]
+
+theorem FLCtx.PSubst.cmp
+  {L₁ L₂ : FLCtx κ ν (Ty α)} {σ : USubst φ ν} {K₁ K₂ : FLCtx κ ν (Ty α)}
+  (hσ₁ : L₁.PSubst σ K₁) (hσ₂ : L₂.PSubst σ K₂) (hL : L₁.Cmp L₂) : K₁.Cmp K₂
+  := λx => (hσ₁ x).cmp (hσ₂ x) (hL x)
 
 def FLCtx.PSubst.toSubst {L : FLCtx κ ν (Ty α)} {σ : USubst φ ν} {K : FLCtx κ ν (Ty α)}
   (hσ : L.PSubst σ K) : L.Subst σ K
@@ -110,6 +152,8 @@ def FCtx.Subst.toPSingleton {Γ : FCtx ν (Ty α)} {σ : USubst φ ν} {Δ : FCt
       simp only [toSingleton, h, FLCtx.singleton_app, ↓reduceIte]
       constructor
 
+-- TODO: use LEq lore
+
 -- def UTerminator.FWfM.subst {Γ : FCtx ν (Ty α)} {t : UTerminator φ ν κ}
 --   (hσ : Γ.Subst σ Δ)
 --   : t.FWfM Δ L → (L' : FLCtx κ ν (Ty α)) × (t.rewrite σ).FWfM Γ L' × (L'.PSubst σ L)
@@ -118,10 +162,6 @@ def FCtx.Subst.toPSingleton {Γ : FCtx ν (Ty α)} {σ : USubst φ ν} {Δ : FCt
 --     let ⟨Ls', ds', σs'⟩ := ds.subst hσ;
 --     let ⟨Lt', dt', σt'⟩ := dt.subst hσ;
 --     ⟨_, ite (de.subst hσ) ds' dt' sorry rfl, σs'.lsup σt'⟩
-
--- TODO: PSubst for FWfM
-
--- TODO: refactor to dePSubst, and so on...
 
 -- def UTerminator.FWf.subst {Γ : FCtx ν (Ty α)} {t : UTerminator φ ν κ}
 --   (hσ : Γ.Subst σ Δ)
